done/Iron/Language/SystemF2Effect/Store/StoreP.v
@@ -11,7 +11,9 @@ Require Export Iron.Language.SystemF2Effect.Store.Bind.
    dangling references into that region. *)
 
 Definition STOREP  (sp : stprops) (fs : stack)
- := forall n, In (FPriv n) fs -> In (SRegion n) sp.
+ := (forall p,     In (FPriv p)    fs -> In (SRegion p)  sp)
+ /\ (forall p1 p2, In (FExt p1 p2) fs -> In (SRegion p1) sp)
+ /\ (forall p1 p2, In (FExt p1 p2) fs -> In (SRegion p2) sp).
 
 
 (* Weaken frame stack in store properties. *)
@@ -20,20 +22,40 @@ Lemma storep_snoc
  ,  STOREP sp fs
  -> STOREP (SRegion p <: sp) (fs :> FPriv p).
 Proof.
- unfold STOREP in *.
- - intros.
-   have HN: (n = p \/ ~(n = p)).
+ unfold STOREP in *. rip.
+
+ - have HN: (p0 = p \/ ~(p0 = p)).
    inverts HN.
-   + rrwrite (  SRegion p <: sp 
-             = (SRegion p <: nil) >< sp).
+   + rrwrite (SRegion p <: sp = (SRegion p <: nil) >< sp).
      snorm.
-   + assert (In (FPriv n) fs).
+   + assert (In (FPriv p0) fs).
       eapply in_tail.
-      have (FPriv n <> FPriv p) by congruence.
+      have (FPriv p0 <> FPriv p) by congruence.
       eauto. auto.
-     rrwrite (  SRegion p <: sp
-             = (SRegion p <: nil) >< sp).
+     rrwrite (SRegion p <: sp = (SRegion p <: nil) >< sp).
      snorm.
+
+ - have HN: (p1 = p \/ ~(p1 = p)).
+   inverts HN.
+   + rrwrite (SRegion p <: sp = (SRegion p <: nil) >< sp).
+     snorm.
+   + assert (In (FExt p1 p2) fs).
+      eapply in_tail.
+      have (FExt p1 p2 <> FPriv p) by congruence. 
+      eauto. auto.
+     rrwrite (SRegion p <: sp = (SRegion p <: nil) >< sp).
+     snorm. eauto.
+
+ - have HN: (p2 = p \/ ~(p2 = p)).
+   inverts HN.
+   + rrwrite (SRegion p <: sp = (SRegion p <: nil) >< sp).
+     snorm.
+   + assert (In (FExt p1 p2) fs).
+      eapply in_tail.
+      have (FExt p1 p2 <> FPriv p) by congruence. 
+      eauto. auto.
+     rrwrite (SRegion p <: sp = (SRegion p <: nil) >< sp).
+     snorm. eauto.
 Qed.
 Hint Resolve storep_snoc.
 
@@ -43,7 +65,9 @@ Lemma storep_stprops_snoc
  ,  STOREP sp fs
  -> STOREP (p <: sp) fs.
 Proof.
- unfold STOREP in *.
- snorm.
+ unfold STOREP in *. rip.
+ - have (In (SRegion p1) sp). snorm.
+ - have (In (SRegion p2) sp). snorm.
 Qed.
 Hint Resolve storep_stprops_snoc.
+
