done/Iron/Language/SystemF2Effect/Step/Frame.v
@@ -6,23 +6,33 @@ Require Export Iron.Language.SystemF2Effect.Store.Prop.
 
 
 (********************************************************************)
-(* Frame Stacks *)
+(* Frames *)
 Inductive frame : Set :=
  (* Holds the continuation of a let-expression while the right
     of the binding is being evaluated. *)
  | FLet   : ty  -> exp      -> frame
 
  (* Private region. *)
- | FPriv  : nat -> frame.
-Hint Constructors frame.
+ | FPriv  : nat -> frame
 
-Definition stack := list frame.
-Hint Unfold stack.
+ (* Region extension.
+    The first region is being extended with the second. *)
+ | FExt   : nat -> nat -> frame.
+Hint Constructors frame.
 
 
 Definition isFPriv (p : nat) (f : frame)
  := f = FPriv p.
 Hint Unfold isFPriv.
+
+
+Definition isFExt  (p1 p2 : nat) (f : frame)
+ := f = FExt p1 p2.
+
+
+(* Frame stacks *)
+Definition stack := list frame.
+Hint Unfold stack.
 
 
 (********************************************************************)
@@ -57,14 +67,27 @@ Inductive
  | SfPrivatePush
    :  forall ss sp fs x p
    ,  p = allocRegion sp
-   -> STEPF  ss sp                 fs             (XPrivate x)
-             ss (SRegion p <: sp) (fs :> FPriv p) (substTX 0 (TRgn p) x)
+   -> STEPF  ss sp                 fs              (XPrivate x)
+             ss (SRegion p <: sp) (fs :> FPriv p)  (substTX 0 (TRgn p) x)
 
- (* Pop a region from the stack. *)
+ (* Pop the frame for a private region and delete it from the heap. *)
  | SfPrivatePop
    :  forall ss sp  fs v1 p
    ,  STEPF  ss                      sp (fs :> FPriv p)(XVal v1)
              (map (deallocate p) ss) sp  fs            (XVal v1)
+
+ (* Begin extending an existing region. *)
+ | SfExtendPush
+   :  forall ss sp fs x p1 p2
+   ,  p2 = allocRegion sp
+   -> STEPF ss sp                  fs                (XExtend (TRgn p1) x)
+            ss (SRegion p2 <: sp) (fs :> FExt p1 p2) (substTX 0 (TRgn p2) x)
+
+ (* Pop the frame for a region extension and merge it with the existing one. *)
+ | SfExtendPop
+   :  forall ss sp fs p1 p2 v1
+   ,  STEPF  ss                      sp (fs :> FExt p1 p2) (XVal v1)
+             (map (mergeB p1 p2) ss) sp fs                 (XVal v1)
 
  (* Store operators *****************************)
  (* Allocate a reference. *) 
